add notion of preorder and closure in Utils.fst: now stable is also for relation, not just preorder

fstar/Main.fst
@@ -1,10 +1,253 @@
 module Main
 
-open Monotonic.ST
+open LowStar.BufferOps
 
-type test_type = | X0 | X1
+module B = LowStar.Buffer
+module HS = FStar.HyperStack
+module G = FStar.Ghost
+module L = FStar.List.Tot
+module U32 = FStar.UInt32
+module MO = LowStar.Modifies
 
-let square (x: UInt32.t): UInt32.t =
-  let open FStar.UInt32 in
-  x *%^ x
+open FStar.HyperStack.ST
+
+#set-options "--__no_positivity"
+
+noeq type t (a:Type0) =
+  B.pointer_or_null (cell a)
+
+and cell (a: Type0) = {
+  next: t a;
+  data: a
+}
+
+let rec well_formed #a (h:HS.mem) (c:t a) (l:G.erased (list a)) :
+  GTot Type0 (decreases (G.reveal l))
+  = B.live h c /\ (
+  match G.reveal l with
+  | [] -> B.g_is_null c
+  | a :: q ->
+    B.length c == 1 /\ (
+      let {data = data; next = next} = B.get h c 0 in
+      a == data /\ well_formed h next (G.hide q)
+    )
+  )
+
+let rec length_functional #a (h:HS.mem) (c:t a) (l1 l2:G.erased (list a)) :
+  Lemma
+    (requires well_formed h c l1 /\ well_formed h c l2)
+    (ensures l1 == l2)
+    (decreases G.reveal l1)
+    [SMTPat (well_formed h c l1); SMTPat (well_formed h c l2)] =
+  if B.g_is_null c then ()
+  else
+    let {next = next} = B.get h c 0 in
+    length_functional h next (G.hide (L.tl (G.reveal l1))) (G.hide (L.tl (G.reveal l2)))
+
+#set-options "--max_ifuel 1 --max_fuel 2"
+val footprint: (#a: Type) -> (h: HS.mem) -> (l: t a) -> (n: G.erased (list a)) -> Ghost MO.loc
+  (requires (well_formed h l n))
+  (ensures (fun refs -> True))
+  (decreases (G.reveal n))
+
+let rec footprint #a h l n =
+  if B.g_is_null l
+  then MO.loc_none
+  else
+    let {next = next} = B.get h l 0 in
+    let refs = footprint h next (G.hide (L.tl (G.reveal n))) in
+    MO.loc_union (MO.loc_buffer l) refs
+#reset-options
+
+let rec modifies_disjoint_footprint
+  (#a: Type)
+  (h: HS.mem)
+  (l: t a)
+  (n: G.erased (list a))
+  (r: MO.loc)
+  (h' : HS.mem)
+: Lemma
+  (requires (
+    well_formed h l n /\
+    MO.loc_disjoint r (footprint h l n) /\
+    MO.modifies r h h'
+  ))
+  (ensures (
+    well_formed h' l n /\
+    footprint h' l n == footprint h l n
+  ))
+  (decreases (G.reveal n))
+= if B.g_is_null l
+  then ()
+  else begin
+    let {next = l'} = B.get h l 0 in
+    modifies_disjoint_footprint h l' (G.hide (L.tl (G.reveal n))) r h'
+  end
+
+let rec well_formed_distinct_lengths_disjoint
+  #a
+  (c1: B.pointer (cell a))
+  (c2: B.pointer (cell a))
+  (n1: G.erased (list a))
+  (n2: G.erased (list a))
+  (h: HS.mem)
+: Lemma
+  (requires (
+    well_formed h c1 n1 /\
+    well_formed h c2 n2 /\
+    L.length (G.reveal n1) <> L.length (G.reveal n2)
+  ))
+  (ensures (
+    B.disjoint c1 c2
+  ))
+  (decreases (L.length (G.reveal n1) + L.length (G.reveal n2)))
+= let {next = next1} = B.get h c1 0 in
+  let {next = next2} = B.get h c2 0 in
+  let f () : Lemma (next1 =!= next2) =
+    if B.g_is_null next1 || B.g_is_null next2
+    then ()
+    else
+      well_formed_distinct_lengths_disjoint next1 next2 (G.hide (L.tl (G.reveal n1))) (G.hide (L.tl (G.reveal n2))) h
+  in
+  f ();
+  B.pointer_distinct_sel_disjoint c1 c2 h
+
+let rec well_formed_gt_lengths_disjoint_from_list
+  #a
+  (h: HS.mem)
+  (c1: B.pointer_or_null (cell a))
+  (c2: B.pointer_or_null (cell a))
+  (n1: G.erased (list a))
+  (n2: G.erased (list a))
+: Lemma
+  (requires (well_formed h c1 n1 /\ well_formed h c2 n2 /\ L.length (G.reveal n1) > L.length (G.reveal n2)))
+  (ensures (MO.loc_disjoint (MO.loc_buffer c1) (footprint h c2 n2)))
+  (decreases (G.reveal n2))
+= match G.reveal n2 with
+  | [] -> ()
+  | _ ->
+    well_formed_distinct_lengths_disjoint c1 c2 n1 n2 h;
+    well_formed_gt_lengths_disjoint_from_list h c1 (B.get h c2 0).next n1 (G.hide (L.tl (G.reveal n2)))
+
+let well_formed_head_tail_disjoint
+  (#a: Type)
+  (h: HS.mem)
+  (c: B.pointer (cell a))
+  (n: G.erased (list a))
+: Lemma
+  (requires (well_formed h c n))
+  (ensures (
+    MO.loc_disjoint (MO.loc_buffer c) (footprint h (B.get h c 0).next (G.hide (L.tl (G.reveal n))))
+  ))
+= well_formed_gt_lengths_disjoint_from_list h c (B.get h c 0).next n (G.hide (L.tl (G.reveal n)))
+
+let rec unused_in_well_formed_disjoint_from_list
+  #a #b
+  (h: HS.mem)
+  (r: B.buffer a)
+  (l: B.pointer_or_null (cell b))
+  (n: G.erased (list b))
+: Lemma
+  (requires (r `B.unused_in` h /\ well_formed h l n))
+  (ensures (MO.loc_disjoint (MO.loc_buffer r) (footprint h l n)))
+  (decreases (G.reveal n))
+= match G.reveal n with
+  | [] -> ()
+  | _ -> unused_in_well_formed_disjoint_from_list h r (B.get h l 0).next (G.hide (L.tl (G.reveal n)))
+
+
+
+val pop: (#a: Type) -> (#n: G.erased (list a)) -> (pl: B.pointer (t a)) ->
+  Stack a
+  (requires (fun h ->
+    let l = B.get h pl 0 in
+    B.live h pl /\
+    well_formed h l n /\
+    MO.loc_disjoint (MO.loc_buffer pl) (footprint h l n) /\
+    Cons? (G.reveal n)
+  ))
+  (ensures (fun h0 v h1 ->
+    let l = B.get h1 pl 0 in
+    let n' = G.hide (L.tl (G.reveal n)) in
+    B.live h1 pl /\
+    MO.modifies (MO.loc_buffer pl) h0 h1 /\
+    well_formed h1 l n' /\
+    MO.loc_disjoint (MO.loc_buffer pl) (footprint h1 l n')
+  ))
+
+let pop #a #n pl =
+  let l = !* pl in
+  let lcell = !* l in
+  let h0 = get () in
+  pl *= lcell.next;
+  let h1 = get () in
+  well_formed_head_tail_disjoint h0 l n;
+  modifies_disjoint_footprint h0 l n (MO.loc_buffer pl) h1;
+  lcell.data
+
+val push: (#a: Type) -> (#n: G.erased (list a)) -> (pl: B.pointer (t a)) -> (x: a) ->
+  ST unit
+    (requires (fun h ->
+      let l = B.get h pl 0 in
+      B.live h pl /\
+      well_formed h l n /\
+      MO.loc_disjoint (MO.loc_buffer pl) (footprint h l n)
+    ))
+    (ensures (fun h0 _ h1 ->
+      let n' = G.hide (x :: G.reveal n) in
+      let l = B.get h1 pl 0 in
+      MO.modifies (MO.loc_buffer pl) h0 h1 /\
+      B.live h1 pl /\
+      well_formed h1 l n' /\
+      MO.loc_disjoint (MO.loc_buffer pl) (footprint h1 l n')
+    ))
+
+let push #a #n pl x =
+  let h0 = get () in
+  let l = !* pl in
+  let c = {
+    data = x;
+    next = l;
+  }
+  in
+  let pc: B.pointer (cell a) = B.malloc HS.root c 1ul in
+  unused_in_well_formed_disjoint_from_list h0 pc l n;
+  let h1 = get () in
+  modifies_disjoint_footprint h0 l n (MO.loc_buffer pc) h1;
+  pl *= pc;
+  let h2 = get () in
+  modifies_disjoint_footprint h1 l n (MO.loc_buffer pl) h2
+
+
+val length (#a: Type) (gn: G.erased (list a)) (l: t a): Stack UInt32.t
+  (requires (fun h -> well_formed h l gn))
+  (ensures (fun h0 n h1 ->
+    h0 == h1 /\
+    U32.v n = L.length (G.reveal gn)
+  ))
+
+let rec length #a gn l =
+  if B.is_null l
+  then 0ul
+  else
+    let open U32 in
+    let c = !* l in
+    let next = c.next in
+    let n = length (G.hide (L.tail (G.reveal gn))) next in
+    if n = 0xfffffffful then begin
+      C.String.(print !$"Integer overflow while computing length");
+      C.exit 255l;
+      0ul // dummy return value, this point is unreachable
+    end else
+      n +^ 1ul
+
+val main: unit -> ST (Int32.t) (fun _ -> true) (fun _ _ _ -> true)
+
+let main () =
+  let l: B.pointer_or_null (t Int32.t) = B.malloc HS.root B.null 1ul in
+  push #Int32.t #(G.hide []) l 1l;
+  push #Int32.t #(G.hide [1l]) l 0l;
+  let r = pop #Int32.t #(G.hide [0l; 1l]) l in
+  TestLib.checku32 (length (G.hide [1l]) !*l) 1ul;
+  r
 
