fstar/MMIO.fst
@@ -1,0 +1,21 @@
+module MMIO
+
+/// definition of MMIO memory region
+module M = FStar.Map
+module U16 = FStar.UInt16
+module U8 = FStar.UInt8
+open Utils
+
+
+// represent a mmio of n bits
+let mmio' (n:nat) = M.t (fin n) bool
+
+let sel' (#n:nat) (addr:mmio' n) (x:fin n) : bool
+    = M.sel addr x
+
+let upd' (#n:nat) (addr:mmio' n) (x:fin n) (b:bool) : mmio' n
+  = M.upd addr x b
+
+let sel_update_lemma' (#n:nat) (addr:mmio' n) (x y:fin n) (b:bool) :
+  Lemma (sel' (upd' addr x b) y == (if x = y then b else sel' addr y))
+  = ()
