fstar/RG.fst
@@ -1,0 +1,7 @@
+module RG
+
+module Map = FStar.Map
+module P = FStar.Preorder
+
+let st_pre (state:Type0) (rely guarantee:P.relation state) =
+  p:(state -> Type0){P.stable p rely}
