fstar/Utils.fst
@@ -1,0 +1,49 @@
+module Utils
+
+module RT = FStar.ReflexiveTransitiveClosure
+
+let fin (n:nat) = x:nat{x < n}
+
+let get_some #a (x: (option a){Some? x})=
+    match x with
+    | Some _x -> _x
+
+let relation (a:Type) = a -> a -> Type0
+let predicate (a:Type) = a -> Type0
+
+
+let stable (#a:Type) (p:predicate a) (r:relation a) : Type0 =
+  forall x y. p x /\ r x y ==> p y
+
+let reflexive (#a:Type) (r:relation a) : Type0 =
+  forall x. r x x
+
+let transitive (#a:Type) (r:relation a) : Type0 =
+  forall x y z. r x y /\ r y z ==> r x z
+
+let preorder (a:Type) : Type =
+  r:relation a{reflexive r /\ transitive r}
+
+
+val closure (#a:Type) (r:a -> a -> Type0) : preorder a
+let closure #a r x y =RT.closure r x y
+
+let closure_step (#a:Type) (r:a -> a -> Type0) (x y:a) :
+  Lemma
+    (requires r x y)
+    (ensures closure r x y)
+    [SMTPat (closure r x y)]
+  = ()
+
+let closure_inversion (#a:Type) (r:a -> a -> Type0) (x y:a) :
+  Lemma 
+    (requires closure r x y)
+    (ensures x == y \/ (exists z. r x z /\ closure r z y))
+  = RT.closure_inversion r x y
+
+let stable_on_closure (#a:Type) (r:a -> a -> Type0) (p:a -> prop) :
+  Lemma
+    (requires forall x y.{:pattern (p y); (r x y)} p x /\ r x y ==> p y)
+    (ensures forall x y.{:pattern (closure r x y)} p x /\ closure r x y ==> p y)
+  = RT.stable_on_closure r p ()
+
