fstar/utils.fst
@@ -1,3 +1,0 @@
-let get_some #a (x: (option a){Some? x})=
-    match x with
-    | Some _x -> _x
